Implement F* envs using Functional Extensionality

rupicola/EquivRel.fsti
@@ -52,7 +52,7 @@ let lem_gsubst_empty (e:closed_exp) : Lemma (gsubst gsub_empty e == e)
   [SMTPat (gsubst gsub_empty e)] =
   admit ()
 
-(** F* Evaluation Environment **)
+(** F* Evaluation Environment : variable -> value **)
 
 (** CA: this is an abstraction that helps with dealing with variables.
    It is like a symbol we introduce when dealing with lambdas and eliminate when dealing with variables **)
@@ -64,7 +64,7 @@ let lem_inverse (g_card:nat) (x:var{x < g_card}) : Lemma (fs_to_var g_card (var_
 let lem_inverse' (g_card:nat) (i:var{i < g_card}) : Lemma (var_to_fs g_card (fs_to_var g_card i) == i) = ()
 
 
-type fs_env #g (g_card:env_card g) : Type u#1000 (** having such an env is even possible in practice? what would its universe be? **)
+val fs_env #g (g_card:env_card g) : Type u#0 (** having such an env is even possible in practice? what would its universe be? **)
 val fs_empty : fs_env #empty 0
 val get_v : #g:_ -> #g_card:env_card g -> fs_env g_card -> i:nat{i < g_card} -> elab_typ (Some?.v (g (fs_to_var g_card i)))
 val fs_extend : #g:_ -> #g_card:env_card g -> fs_s:fs_env g_card -> #t:typ -> elab_typ t -> fs_s':(fs_env #(extend t g) (g_card+1))
@@ -79,7 +79,7 @@ val lem_fs_shrink #g (#g_card:env_card g) #t (fs_s:fs_env #(extend t g) (g_card+
   (forall (i:nat). i < g_card ==> get_v fs_s i == get_v (fs_shrink fs_s) i))
   [SMTPat (fs_shrink fs_s)]
 
-val pop_extend_inverse #g (#g_card:env_card g) (fs_s:fs_env g_card) #t (x:elab_typ t) : Lemma (fs_shrink (fs_extend fs_s x) == fs_s)
+val shrink_extend_inverse #g (#g_card:env_card g) (fs_s:fs_env g_card) #t (x:elab_typ t) : Lemma (fs_shrink (fs_extend fs_s x) == fs_s)
   [SMTPat (fs_shrink (fs_extend fs_s x))]
 
 let (∽) (#g:env) #b #g_card (s:gsub g g_card b) (fs_s:fs_env g_card) : Type0 =
