rupicola/EquivRel.fst
@@ -1,0 +1,38 @@
+module EquivRel
+
+open FStar.FunctionalExtensionality
+
+type fs_env #g g_card =
+  restricted_t (x:var{x < g_card}) (fun x -> elab_typ (Some?.v (g x)))
+
+let fs_empty : fs_env #empty 0 =
+  on_dom
+    (x:var{x < 0})
+    #(fun x -> elab_typ (Some?.v (empty x)))
+    (fun _ -> assert False)
+
+let get_v #g #g_card fs_s i =
+  fs_s (fs_to_var g_card i)
+
+let fs_extend #g #g_card fs_s #t fs_v =
+  on_dom
+    (x:var{x < g_card+1})
+    #(fun x -> elab_typ (Some?.v ((extend t g) x)))
+    (fun y ->
+      if y = 0 then fs_v else fs_s (y-1))
+
+let fs_shrink #t #g #g_card fs_s =
+  on_dom
+    (x:var{x < g_card})
+    #(fun x -> elab_typ (Some?.v (g x)))
+    (fun y -> fs_s (y+1))
+
+let lem_fs_extend fs_s v = ()
+let lem_fs_shrink fs_s = ()
+
+let shrink_extend_inverse #g #g_card fs_s #t v =
+  let fs_s' : fs_env g_card = fs_shrink (fs_extend fs_s v) in
+  assert (forall x. fs_s' x == fs_s x);
+  assert (feq fs_s' fs_s);
+  extensionality _ _ fs_s' fs_s;
+  assert (fs_s' == fs_s)
